Partially_Filled_Array.thy
@@ -15,12 +15,12 @@ type_synonym 'a pfarray = "'a array_list"
 section "Operations on Partly Filled Arrays"
 
 
-definition is_pfarray_cap where
-  "is_pfarray_cap c l \<equiv> \<lambda>(a,n). \<exists>\<^sub>A l'. a \<mapsto>\<^sub>a l' *  \<up>(c = length l' \<and> n \<le> c \<and> l = (take n l'))"
+definition is_pfa where
+  "is_pfa c l \<equiv> \<lambda>(a,n). \<exists>\<^sub>A l'. a \<mapsto>\<^sub>a l' *  \<up>(c = length l' \<and> n \<le> c \<and> l = (take n l'))"
 
 
-lemma is_pfarray_cap_prec[safe_constraint_rules]: "precise (is_pfarray_cap c)"
-  unfolding is_pfarray_cap_def[abs_def]
+lemma is_pfa_prec[safe_constraint_rules]: "precise (is_pfa c)"
+  unfolding is_pfa_def[abs_def]
   apply(rule preciseI)
   apply(simp split: prod.splits) 
   using preciseD snga_prec by fastforce
@@ -31,25 +31,25 @@ definition pfa_init where
   return (a,n)
 }"
 
-lemma pfa_init_rule[sep_heap_rules]: "n \<le> N \<Longrightarrow> < emp > pfa_init N x n <is_pfarray_cap N (replicate n x)>"
-  by (sep_auto simp: pfa_init_def is_pfarray_cap_def)
+lemma pfa_init_rule[sep_heap_rules]: "n \<le> N \<Longrightarrow> < emp > pfa_init N x n <is_pfa N (replicate n x)>"
+  by (sep_auto simp: pfa_init_def is_pfa_def)
 
 definition pfa_empty where
   "pfa_empty cap \<equiv> pfa_init cap default 0"
 
 
 
-lemma pfa_empty_rule[sep_heap_rules]: "< emp > pfa_empty N <is_pfarray_cap N []>"
-  by (sep_auto simp: pfa_empty_def is_pfarray_cap_def)
+lemma pfa_empty_rule[sep_heap_rules]: "< emp > pfa_empty N <is_pfa N []>"
+  by (sep_auto simp: pfa_empty_def is_pfa_def)
 
 
 definition "pfa_length \<equiv> arl_length"
 
 lemma pfa_length_rule[sep_heap_rules]: "
-  <is_pfarray_cap c l a> 
+  <is_pfa c l a> 
     pfa_length a
-  <\<lambda>r. is_pfarray_cap c l a * \<up>(r=length l)>"
-  by (sep_auto simp: pfa_length_def arl_length_def is_pfarray_cap_def)
+  <\<lambda>r. is_pfa c l a * \<up>(r=length l)>"
+  by (sep_auto simp: pfa_length_def arl_length_def is_pfa_def)
 
 
 definition "pfa_capacity \<equiv> \<lambda>(a,n). Array.len a
@@ -57,20 +57,20 @@ definition "pfa_capacity \<equiv> \<lambda>(a,n). Array.len a
 
 
 lemma pfa_capacity_rule[sep_heap_rules]: "
-  <is_pfarray_cap c l a> 
+  <is_pfa c l a> 
     pfa_capacity a
-  <\<lambda>r. is_pfarray_cap c l a * \<up>(c=r)>"
-  by (sep_auto simp: pfa_capacity_def arl_length_def is_pfarray_cap_def)
+  <\<lambda>r. is_pfa c l a * \<up>(c=r)>"
+  by (sep_auto simp: pfa_capacity_def arl_length_def is_pfa_def)
 
 
 
 definition "pfa_is_empty \<equiv> arl_is_empty"
 
 lemma pfa_is_empty_rule[sep_heap_rules]: "
-  <is_pfarray_cap c l a> 
+  <is_pfa c l a> 
     pfa_is_empty a
-  <\<lambda>r. is_pfarray_cap c l a * \<up>(r\<longleftrightarrow>(l=[]))>"
-  by (sep_auto simp: pfa_is_empty_def arl_is_empty_def is_pfarray_cap_def)
+  <\<lambda>r. is_pfa c l a * \<up>(r\<longleftrightarrow>(l=[]))>"
+  by (sep_auto simp: pfa_is_empty_def arl_is_empty_def is_pfa_def)
 
 
 
@@ -81,11 +81,11 @@ definition "pfa_append \<equiv> \<lambda>(a,n) x. do {
 
 lemma pfa_append_rule[sep_heap_rules]: "
    n < c  \<Longrightarrow>
-    < is_pfarray_cap c l (a,n) > 
+    < is_pfa c l (a,n) > 
       pfa_append (a,n) x 
-    <\<lambda>(a',n'). is_pfarray_cap c (l@[x]) (a',n') * \<up>(a' = a \<and> n' = n+1) >"  
+    <\<lambda>(a',n'). is_pfa c (l@[x]) (a',n') * \<up>(a' = a \<and> n' = n+1) >"  
   by (sep_auto 
-      simp: pfa_append_def arl_append_def is_pfarray_cap_def take_update_last neq_Nil_conv
+      simp: pfa_append_def arl_append_def is_pfa_def take_update_last neq_Nil_conv
       split: prod.splits nat.split)
 
 
@@ -94,10 +94,10 @@ definition "pfa_last \<equiv> arl_last"
 
 lemma pfa_last_rule[sep_heap_rules]: "
   l\<noteq>[] \<Longrightarrow>
-  <is_pfarray_cap c l a> 
+  <is_pfa c l a> 
     pfa_last a
-  <\<lambda>r. is_pfarray_cap c l a * \<up>(r=last l)>"
-  by (sep_auto simp: pfa_last_def arl_last_def is_pfarray_cap_def last_take_nth_conv)
+  <\<lambda>r. is_pfa c l a * \<up>(r=last l)>"
+  by (sep_auto simp: pfa_last_def arl_last_def is_pfa_def last_take_nth_conv)
 
 
 definition pfa_butlast :: "'a::heap pfarray \<Rightarrow> 'a pfarray Heap" where
@@ -107,32 +107,32 @@ definition pfa_butlast :: "'a::heap pfarray \<Rightarrow> 'a pfarray Heap" where
 
 
 lemma pfa_butlast_rule[sep_heap_rules]: "
-  <is_pfarray_cap c l (a,n)> 
+  <is_pfa c l (a,n)> 
     pfa_butlast (a,n)
-  <\<lambda>(a',n'). is_pfarray_cap c (butlast l) (a',n') * \<up>(a' = a)>"
+  <\<lambda>(a',n'). is_pfa c (butlast l) (a',n') * \<up>(a' = a)>"
   by (sep_auto 
       split: prod.splits
-      simp: pfa_butlast_def is_pfarray_cap_def butlast_take)  
+      simp: pfa_butlast_def is_pfa_def butlast_take)  
 
 
 definition "pfa_get \<equiv> arl_get"
 
 lemma pfa_get_rule[sep_heap_rules]: "
   i < length l \<Longrightarrow>
-  < is_pfarray_cap c l a> 
+  < is_pfa c l a> 
     pfa_get a i
-  <\<lambda>r. is_pfarray_cap c l a * \<up>((l!i) = r)>"
-  by (sep_auto simp: is_pfarray_cap_def pfa_get_def arl_get_def  split: prod.split)
+  <\<lambda>r. is_pfa c l a * \<up>((l!i) = r)>"
+  by (sep_auto simp: is_pfa_def pfa_get_def arl_get_def  split: prod.split)
 
 
 definition "pfa_set \<equiv> arl_set"
 
 lemma pfa_set_rule[sep_heap_rules]: "
     i<length l \<Longrightarrow>
-    <is_pfarray_cap c l a> 
+    <is_pfa c l a> 
       pfa_set a i x
-    <\<lambda>a'. is_pfarray_cap c (l[i:=x]) a' * \<up>(a' = a)>"
-  by (sep_auto simp: pfa_set_def arl_set_def is_pfarray_cap_def split: prod.split)
+    <\<lambda>a'. is_pfa c (l[i:=x]) a' * \<up>(a' = a)>"
+  by (sep_auto simp: pfa_set_def arl_set_def is_pfa_def split: prod.split)
 
 
 
@@ -146,11 +146,11 @@ definition pfa_shrink :: "nat \<Rightarrow> 'a::heap pfarray \<Rightarrow> 'a pf
 
 lemma pfa_shrink_rule[sep_heap_rules]: "
    k \<le> length l \<Longrightarrow>
-    < is_pfarray_cap c l (a,n) > 
+    < is_pfa c l (a,n) > 
       pfa_shrink k (a,n)
-    <\<lambda>(a',n'). is_pfarray_cap c (take k l) (a',n') * \<up>(n' = k \<and> a'=a) >"  
+    <\<lambda>(a',n'). is_pfa c (take k l) (a',n') * \<up>(n' = k \<and> a'=a) >"  
   by (sep_auto 
-      simp: pfa_shrink_def is_pfarray_cap_def min.absorb1
+      simp: pfa_shrink_def is_pfa_def min.absorb1
       split: prod.splits nat.split)
 
 
@@ -163,22 +163,22 @@ definition pfa_shrink_cap :: "nat \<Rightarrow> 'a::heap pfarray \<Rightarrow> '
 
 lemma pfa_shrink_cap_rule_preserve[sep_heap_rules]: "
    \<lbrakk>n \<le> k; k \<le> c\<rbrakk> \<Longrightarrow>
-    < is_pfarray_cap c l (a,n) > 
+    < is_pfa c l (a,n) > 
       pfa_shrink_cap k (a,n)
-    <\<lambda>a'. is_pfarray_cap k l a' >\<^sub>t"
+    <\<lambda>a'. is_pfa k l a' >\<^sub>t"
   by (sep_auto 
-      simp: pfa_shrink_cap_def is_pfarray_cap_def min.absorb1 min.absorb2
+      simp: pfa_shrink_cap_def is_pfa_def min.absorb1 min.absorb2
       split: prod.splits nat.split)
 
 
 
 lemma pfa_shrink_cap_rule: "
    \<lbrakk>k \<le> c\<rbrakk> \<Longrightarrow>
-    < is_pfarray_cap c l a > 
+    < is_pfa c l a > 
       pfa_shrink_cap k a
-    <\<lambda>a'. is_pfarray_cap k (take k l) a' >\<^sub>t"  
+    <\<lambda>a'. is_pfa k (take k l) a' >\<^sub>t"  
   by (sep_auto 
-      simp: pfa_shrink_cap_def is_pfarray_cap_def min.absorb1 min.absorb2
+      simp: pfa_shrink_cap_def is_pfa_def min.absorb1 min.absorb2
       split: prod.splits nat.split dest: mod_starD)
 
 
@@ -210,21 +210,21 @@ definition pfa_ensure :: "'a::{heap,default} pfarray \<Rightarrow> nat \<Rightar
 "
 
 lemma pfa_ensure_rule[sep_heap_rules]: "
-    < is_pfarray_cap c l (a,n) > 
+    < is_pfa c l (a,n) > 
       pfa_ensure (a,n) k
-    <\<lambda>(a',n'). is_pfarray_cap (max c k) l (a',n') * \<up>(n' = n \<and> c \<ge> n)>\<^sub>t"  
+    <\<lambda>(a',n'). is_pfa (max c k) l (a',n') * \<up>(n' = n \<and> c \<ge> n)>\<^sub>t"  
   by (sep_auto 
-      simp: pfa_ensure_def is_pfarray_cap_def)
+      simp: pfa_ensure_def is_pfa_def)
 
 
 definition "pfa_copy \<equiv> arl_copy"
 
 
 lemma pfa_copy_rule[sep_heap_rules]:
-  "< is_pfarray_cap c l a >
+  "< is_pfa c l a >
    pfa_copy a
-   <\<lambda>r. is_pfarray_cap c l a * is_pfarray_cap c l r>\<^sub>t"  
-  by (sep_auto simp: pfa_copy_def arl_copy_def is_pfarray_cap_def)
+   <\<lambda>r. is_pfa c l a * is_pfa c l r>\<^sub>t"  
+  by (sep_auto simp: pfa_copy_def arl_copy_def is_pfa_def)
 
 definition pfa_blit :: "'a::heap pfarray \<Rightarrow> nat \<Rightarrow> 'a::heap pfarray \<Rightarrow> nat \<Rightarrow> nat \<Rightarrow> unit Heap" where
   "pfa_blit \<equiv> \<lambda>(src,sn) si (dst,dn) di l. blit src si dst di l"
@@ -237,13 +237,13 @@ lemma min_nat: "min a (a+b) = (a::nat)"
 lemma pfa_blit_rule[sep_heap_rules]:
   assumes LEN: "si+len \<le> sn" "di \<le> dn" "di+len \<le> dc"
   shows
-    "< is_pfarray_cap sc src (srci,sn)
-      * is_pfarray_cap dc dst (dsti,dn) >
+    "< is_pfa sc src (srci,sn)
+      * is_pfa dc dst (dsti,dn) >
     pfa_blit (srci,sn) si (dsti,dn) di len
-    <\<lambda>_. is_pfarray_cap sc src (srci,sn)
-      * is_pfarray_cap dc (take di dst @ take len (drop si src) @ drop (di+len) dst) (dsti,max (di+len) dn)
+    <\<lambda>_. is_pfa sc src (srci,sn)
+      * is_pfa dc (take di dst @ take len (drop si src) @ drop (di+len) dst) (dsti,max (di+len) dn)
     >"
-  using LEN apply(sep_auto simp add: min_nat is_pfarray_cap_def pfa_blit_def min.commute min.absorb1 heap: blit_rule)
+  using LEN apply(sep_auto simp add: min_nat is_pfa_def pfa_blit_def min.commute min.absorb1 heap: blit_rule)
    apply (simp add: min.absorb1 take_drop)
   apply (simp add: drop_take max_def)
   done
@@ -259,14 +259,14 @@ definition pfa_drop :: "('a::heap) pfarray \<Rightarrow> nat \<Rightarrow> 'a pf
 lemma pfa_drop_rule[sep_heap_rules]:
   assumes LEN: "k \<le> sn" "(sn-k) \<le> dc"
   shows
-    "< is_pfarray_cap sc src (srci,sn)
-      * is_pfarray_cap dc dst (dsti,dn) >
+    "< is_pfa sc src (srci,sn)
+      * is_pfa dc dst (dsti,dn) >
     pfa_drop (srci,sn) k (dsti,dn)
-    <\<lambda>(dsti',dn'). is_pfarray_cap sc src (srci,sn)
-      * is_pfarray_cap dc (drop k src) (dsti',dn')
+    <\<lambda>(dsti',dn'). is_pfa sc src (srci,sn)
+      * is_pfa dc (drop k src) (dsti',dn')
       * \<up>(dsti' = dsti)
     >"
-  using LEN apply (sep_auto simp add: drop_take is_pfarray_cap_def pfa_drop_def dest!: mod_starD heap: pfa_blit_rule)
+  using LEN apply (sep_auto simp add: drop_take is_pfa_def pfa_drop_def dest!: mod_starD heap: pfa_blit_rule)
   done
 
 
@@ -281,10 +281,10 @@ definition "pfa_append_grow \<equiv> \<lambda>(a,n) x. do {
 
 
 lemma pfa_append_grow_full_rule[sep_heap_rules]: "n = c \<Longrightarrow>
-     <is_pfarray_cap c l (a,n)>
+     <is_pfa c l (a,n)>
   array_grow a (c+1) x
-      <\<lambda>a'. is_pfarray_cap (c+1) (l@[x]) (a',n+1)>\<^sub>t"
-  apply(sep_auto simp add: is_pfarray_cap_def 
+      <\<lambda>a'. is_pfa (c+1) (l@[x]) (a',n+1)>\<^sub>t"
+  apply(sep_auto simp add: is_pfa_def 
       heap del: array_grow_rule)
   apply(vcg heap del: array_grow_rule heap add: array_grow_rule[of l "(Suc (length l))" a x])
    apply simp
@@ -294,22 +294,22 @@ lemma pfa_append_grow_full_rule[sep_heap_rules]: "n = c \<Longrightarrow>
 
 
 lemma pfa_append_grow_less_rule: "n < c \<Longrightarrow>
- <is_pfarray_cap c l (a,n)>
+ <is_pfa c l (a,n)>
     Array.upd n x a
-<\<lambda>a'. is_pfarray_cap c (l@[x]) (a',n+1)>\<^sub>t"
-  apply(sep_auto simp add: is_pfarray_cap_def take_update_last)
+<\<lambda>a'. is_pfa c (l@[x]) (a',n+1)>\<^sub>t"
+  apply(sep_auto simp add: is_pfa_def take_update_last)
   done
 
 lemma pfa_append_grow_rule[sep_heap_rules]: "
-  <is_pfarray_cap c l (a,n)>
+  <is_pfa c l (a,n)>
   pfa_append_grow (a,n) x 
-  <\<lambda>(a',n'). is_pfarray_cap (if c = n then c+1 else c) (l@[x]) (a',n') * \<up>(n'=n+1 \<and> c \<ge> n)>\<^sub>t"
+  <\<lambda>(a',n'). is_pfa (if c = n then c+1 else c) (l@[x]) (a',n') * \<up>(n'=n+1 \<and> c \<ge> n)>\<^sub>t"
   apply(subst pfa_append_grow_def)
   apply(rule hoare_triple_preI)
   apply (sep_auto
       heap add: pfa_append_grow_full_rule pfa_append_grow_less_rule)
-   apply(sep_auto simp add: is_pfarray_cap_def)
-  apply(sep_auto simp add: is_pfarray_cap_def)
+   apply(sep_auto simp add: is_pfa_def)
+  apply(sep_auto simp add: is_pfa_def)
   done
 
 (* This definition has only one access to the array length *)
@@ -320,9 +320,9 @@ definition "pfa_append_grow' \<equiv> \<lambda>(a,n) x. do {
 }"
 
 lemma pfa_append_grow'_rule[sep_heap_rules]: "
-  <is_pfarray_cap c l (a,n)>
+  <is_pfa c l (a,n)>
   pfa_append_grow' (a,n) x 
-  <\<lambda>(a',n'). is_pfarray_cap (max (n+1) c) (l@[x]) (a',n') * \<up>(n'=n+1 \<and> c \<ge> n)>\<^sub>t"
+  <\<lambda>(a',n'). is_pfa (max (n+1) c) (l@[x]) (a',n') * \<up>(n'=n+1 \<and> c \<ge> n)>\<^sub>t"
   unfolding pfa_append_grow'_def
   by (sep_auto simp add: max_def)
 
@@ -339,10 +339,10 @@ lemma list_update_last: "length ls = Suc i \<Longrightarrow> ls[i:=x] = (take i 
 
 lemma pfa_insert_rule[sep_heap_rules]:
   "\<lbrakk>i \<le> n; n < c\<rbrakk> \<Longrightarrow>
-  <is_pfarray_cap c l (a,n)>
+  <is_pfa c l (a,n)>
   pfa_insert (a,n) i x 
-  <\<lambda>(a',n'). is_pfarray_cap c (take i l@x#drop i l) (a',n') * \<up>(n' = n+1 \<and> a=a')>"
-  unfolding pfa_insert_def is_pfarray_cap_def 
+  <\<lambda>(a',n'). is_pfa c (take i l@x#drop i l) (a',n') * \<up>(n' = n+1 \<and> a=a')>"
+  unfolding pfa_insert_def is_pfa_def 
   by (sep_auto simp add: list_update_append1 list_update_last
       Suc_diff_le drop_take min_def)
 
@@ -355,9 +355,9 @@ definition pfa_insert_grow ::  "'a::{heap,default} pfarray \<Rightarrow> nat \<R
 
 lemma pfa_insert_grow_rule: 
   "i \<le> n \<Longrightarrow>
-  <is_pfarray_cap c l (a,n)>
+  <is_pfa c l (a,n)>
   pfa_insert_grow (a,n) i x 
-  <\<lambda>(a',n'). is_pfarray_cap (max c (n+1)) (take i l@x#drop i l) (a',n') * \<up>(n'=n+1 \<and> c \<ge> n)>\<^sub>t"
+  <\<lambda>(a',n'). is_pfa (max c (n+1)) (take i l@x#drop i l) (a',n') * \<up>(n'=n+1 \<and> c \<ge> n)>\<^sub>t"
   unfolding pfa_insert_grow_def  
   by (sep_auto heap add: pfa_insert_rule[of i n "max c (Suc n)"])
 
@@ -370,11 +370,11 @@ definition pfa_extend where
 
 lemma pfa_extend_rule: 
   "n+m \<le> c \<Longrightarrow>
-  <is_pfarray_cap c l1 (a,n) * is_pfarray_cap d l2 (b,m)>
+  <is_pfa c l1 (a,n) * is_pfa d l2 (b,m)>
   pfa_extend (a,n) (b,m) 
-  <\<lambda>(a',n'). is_pfarray_cap c (l1@l2) (a',n') * \<up>(a' = a \<and> n'=n+m) * is_pfarray_cap d l2 (b,m)>\<^sub>t"
+  <\<lambda>(a',n'). is_pfa c (l1@l2) (a',n') * \<up>(a' = a \<and> n'=n+m) * is_pfa d l2 (b,m)>\<^sub>t"
   unfolding pfa_extend_def  
-  by (sep_auto simp add: is_pfarray_cap_def min.absorb1 min.absorb2 heap add: blit_rule)
+  by (sep_auto simp add: is_pfa_def min.absorb1 min.absorb2 heap add: blit_rule)
 
 
 definition pfa_extend_grow where
@@ -385,11 +385,11 @@ definition pfa_extend_grow where
 }"
 
 lemma pfa_extend_grow_rule: 
-  "<is_pfarray_cap c l1 (a,n) * is_pfarray_cap d l2 (b,m)>
+  "<is_pfa c l1 (a,n) * is_pfa d l2 (b,m)>
   pfa_extend_grow (a,n) (b,m) 
-  <\<lambda>(a',n'). is_pfarray_cap (max c (n+m)) (l1@l2) (a',n') * \<up>(n'=n+m \<and> c \<ge> n) * is_pfarray_cap d l2 (b,m)>\<^sub>t"
+  <\<lambda>(a',n'). is_pfa (max c (n+m)) (l1@l2) (a',n') * \<up>(n'=n+m \<and> c \<ge> n) * is_pfa d l2 (b,m)>\<^sub>t"
   unfolding pfa_extend_grow_def  
-  by (sep_auto simp add: is_pfarray_cap_def min.absorb1 min.absorb2 heap add: blit_rule)
+  by (sep_auto simp add: is_pfa_def min.absorb1 min.absorb2 heap add: blit_rule)
   
 definition pfa_append_extend_grow where
 "pfa_append_extend_grow \<equiv> \<lambda> (a,n) x (b,m). do{
@@ -400,11 +400,11 @@ definition pfa_append_extend_grow where
 }"
 
 lemma pfa_append_extend_grow_rule: 
-  "<is_pfarray_cap c l1 (a,n) * is_pfarray_cap d l2 (b,m)>
+  "<is_pfa c l1 (a,n) * is_pfa d l2 (b,m)>
   pfa_append_extend_grow (a,n) x (b,m) 
-  <\<lambda>(a',n'). is_pfarray_cap (max c (n+m+1)) (l1@x#l2) (a',n') * \<up>(n'=n+m+1 \<and> c \<ge> n) * is_pfarray_cap d l2 (b,m)>\<^sub>t"
+  <\<lambda>(a',n'). is_pfa (max c (n+m+1)) (l1@x#l2) (a',n') * \<up>(n'=n+m+1 \<and> c \<ge> n) * is_pfa d l2 (b,m)>\<^sub>t"
   unfolding pfa_append_extend_grow_def  
-  by (sep_auto simp add: list_update_last is_pfarray_cap_def min.absorb1 min.absorb2 heap add: blit_rule)
+  by (sep_auto simp add: list_update_last is_pfa_def min.absorb1 min.absorb2 heap add: blit_rule)
   
 
 definition "pfa_delete \<equiv> \<lambda>(a,n) i. do {
@@ -414,10 +414,10 @@ definition "pfa_delete \<equiv> \<lambda>(a,n) i. do {
 
 lemma pfa_delete_rule[sep_heap_rules]:
   "i < n \<Longrightarrow>
-  <is_pfarray_cap c l (a,n)>
+  <is_pfa c l (a,n)>
   pfa_delete (a,n) i
-  <\<lambda>(a',n'). is_pfarray_cap c (take i l@drop (i+1) l) (a',n') * \<up>(n' = n-1 \<and> a=a')>"
-  unfolding pfa_delete_def is_pfarray_cap_def 
+  <\<lambda>(a',n'). is_pfa c (take i l@drop (i+1) l) (a',n') * \<up>(n' = n-1 \<and> a=a')>"
+  unfolding pfa_delete_def is_pfa_def 
   apply (sep_auto simp add: drop_take min_def)
   by (metis Suc_diff_Suc diff_zero dual_order.strict_trans2 le_less_Suc_eq zero_le)
 
